Filled some holes

sepcomp/CminorSel_coop.v
@@ -184,43 +184,7 @@ Inductive CMinSel_corestep (ge : genv) : CMinSel_core -> mem ->
   | cminsel_corestep_return: forall v optid f sp e k m,
       CMinSel_corestep ge (CMinSel_Returnstate v (Kcall optid f sp e k)) m
         (CMinSel_State f Sskip k sp (Cminor.set_optvar optid v e)) m.
-(*
-Definition CMinSel_corestep (ge : genv)  (q : CMinSel_core) (m : mem) (q' : CMinSel_core) (m' : mem) : Prop.
-  destruct q; destruct q'.
-  (*State - State*)
-       apply (exists t, step ge (State f s k sp e m)  t (State f0 s0 k0 sp0 e0 m')).
-  (*State - Callstate: one case: step_call*)
-       apply (exists t, step ge (State f s k sp e m)  t (Callstate f0 args k0 m')).
-  (*State - Returnstate - three cases: step_skip_call, step_return_0, step_return_1*)
-       apply (exists t, step ge (State f s k sp e m)  t (Returnstate v k0 m')).
-  (*Callstate - State: only case: step_internal_function*)
-       apply (exists t, step ge (Callstate f args k m) t (State f0 s k0 sp e m')).
-  (*Callstate - Callstate: no case*)
-       apply False.
-  (*Callstate - Returnstate: one case: step_external_function : we don't want this as a step in this semantics, since
-                    stepping should not happen at_external*)
-       apply False.
-  (*Returnstate - State: one case: step_return*)
-       apply (exists t, step ge (Returnstate v k m) t (State f s k0 sp e m')).
-  (*Returnstate - Callstate: no case*)
-       apply False.
-  (*Returnstate - Returnstate: no case*)
-       apply False.
-Defined.
 
-Lemma CMinSel_corestep_not_at_external:
-       forall ge m q m' q', CMinSel_corestep ge q m q' m' -> CMinSel_at_external q = None.
-  Proof. intros.
-     unfold CMinSel_corestep in H. 
-     destruct q; destruct q'; simpl in *; try reflexivity.
-       (*case step_internal_function*)  
-             destruct H as [t Ht]. inversion Ht; subst. reflexivity.
-       (*Call - Call: no case*)
-             contradiction.
-       (*Call - Return: no case in CminorSel_corestep*)
-             contradiction.
-  Qed.
-*)
 Lemma CMinSel_corestep_not_at_external:
        forall ge m q m' q', CMinSel_corestep ge q m q' m' -> CMinSel_at_external q = None.
   Proof. intros. inv H; reflexivity. Qed.
@@ -230,21 +194,6 @@ Definition CMinSel_halted (q : CMinSel_core): option val :=
        CMinSel_Returnstate v Kstop => Some v
      | _ => None
     end.
-(*
-Lemma CMinSel_corestep_not_halted : forall ge m q m' q', 
-       CMinSel_corestep ge q m q' m' -> CMinSel_halted q = None.
-  Proof. intros.
-     unfold CMinSel_corestep in H. 
-     destruct q; destruct q'; simpl in *; try reflexivity.
-          (*case step_return*) 
-             destruct H as [t Ht]. inversion Ht; subst. 
-             destruct v; reflexivity.
-       (*Returnstate - Callstate: no case*)
-             contradiction.
-       (*Returnstate - Returnstate: no case in Cmin_corestep*)
-             contradiction.
-  Qed.
-    *)
 
 Lemma CMinSel_corestep_not_halted : forall ge m q m' q', 
        CMinSel_corestep ge q m q' m' -> CMinSel_halted q = None.
@@ -286,62 +235,10 @@ Definition CMinSel_core_sem : CoreSemantics genv CMinSel_core mem.
     apply CMinSel_after_at_external_excl.
 Defined.
 
-(*
-Lemma CMinSel_corestep_2_CompCertStep: forall (ge : genv)  (q :CMinSel_core) (m : mem) (q' : CMinSel_core) (m' : mem) ,
-   CMinSel_corestep ge q m q' m' -> 
-   exists t, step ge (ToState q m) t (ToState q' m').
-Proof.
-  intros. destruct q; destruct q'; induction H; simpl; eauto. 
-Qed.
+(************************NOW SHOW THAT WE ALSO HAVE A COOPSEM******)
 
-Lemma CompCertStep_CMinSel_corestep: forall (ge : genv)  (q : CMinSel_core) (m : mem) (q' : CMinSel_core) (m' : mem)  t,
-   step ge (ToState q m) t (ToState q' m') ->
-   CMinSel_at_external q = None ->
-   CMinSel_corestep ge q m q' m'.
-Proof.
-  intros. destruct q; destruct q'; simpl in *; try eexists; try eassumption; inv H; discriminate.
-Qed.
-
-Lemma CompCertStep_CMinSel_corestep': forall (ge : genv)  (q : CMinSel_core) (m : mem) c' t q' m',
-   step ge (ToState q m) t c' ->
-   CMinSel_at_external q = None ->
-     q'= fst (FromState c') -> m' = snd (FromState c') -> 
-     CMinSel_corestep ge q m q' m'.
-Proof.
-  intros. assert (c' = ToState q' m'). subst. destruct c'; simpl; trivial.
-  rewrite H3 in H. clear H3. eapply CompCertStep_CMinSel_corestep; eassumption.
-Qed.
-*)
-(*
 Lemma CMinSel_forward : forall g c m c' m' (CS: CMinSel_corestep g c m c' m'), 
-      mem_lemmas.mem_forward m m'.
-  Proof. intros.
-     unfold CMinSel_corestep in CS. 
-     destruct c; destruct c'; simpl in *; try contradiction. 
-       destruct CS as [t CS].
-         inv CS; try apply mem_forward_refl.
-         (*Storev*)
-          destruct vaddr; simpl in H15; inv H15. 
-          eapply store_forward. eassumption. 
-         (*builtin*) 
-          eapply external_call_mem_forward; eassumption.
-       destruct CS as [t CS].
-         inv CS; simpl; try apply mem_forward_refl.
-         (*free*)
-         eapply free_forward; eassumption.
-       destruct CS as [t CS].
-         inv CS; simpl.
-         eapply free_forward; eassumption.
-         eapply free_forward; eassumption.
-         eapply free_forward; eassumption.
-       destruct CS as [t CS].
-         inv CS; simpl. 
-         eapply alloc_forward; eassumption.
-       destruct CS as [t CS].
-         inv CS; simpl. apply mem_forward_refl.
-Qed.*)
-Lemma CMinSel_forward : forall g c m c' m' (CS: CMinSel_corestep g c m c' m'), 
-      mem_lemmas.mem_forward m m'.
+      mem_forward m m'.
   Proof. intros.
      inv CS; try apply mem_forward_refl.
          eapply free_forward; eassumption.
@@ -356,44 +253,8 @@ Lemma CMinSel_forward : forall g c m c' m' (CS: CMinSel_corestep g c m c' m'),
          eapply alloc_forward; eassumption.
 Qed.
 
-Definition coopstep g c m c' m' :=
-   CMinSel_corestep g c m c' m'.
-
-Lemma cminsel_coopstep_not_at_external: forall ge m q m' q',
-  coopstep ge q m q' m' -> CMinSel_at_external q = None.
-Proof.
-  intros.
-  eapply CMinSel_corestep_not_at_external. apply H. 
-Qed.
-
-Lemma cminsel_coopstep_not_halted :
-  forall ge m q m' q', coopstep ge q m q' m' -> CMinSel_halted q = None.
-Proof.
-  intros.
-  eapply CMinSel_corestep_not_halted. apply H.
-Qed.
-
-Program Definition cminsel_core_sem : 
-  CoreSemantics genv CMinSel_core mem :=
-  @Build_CoreSemantics _ _ _ 
-    CMinSel_initial_core
-    CMinSel_at_external
-    CMinSel_after_external
-    CMinSel_halted
-    coopstep
-    cminsel_coopstep_not_at_external
-    cminsel_coopstep_not_halted 
-    CMinSel_at_external_halted_excl
-    CMinSel_after_at_external_excl.
-
-(************************NOW SHOW THAT WE ALSO HAVE A COOPSEM******)
-
-Lemma cminsel_coop_forward : forall g c m c' m' (CS: coopstep g c m c' m'), 
-      mem_lemmas.mem_forward m m'.
-Proof. intros. eapply CMinSel_forward. apply CS. Qed.
-
 Program Definition cminsel_coop_sem : 
   CoopCoreSem genv CMinSel_core.
-apply Build_CoopCoreSem with (coopsem := cminsel_core_sem).
-  apply cminsel_coop_forward.
+apply Build_CoopCoreSem with (coopsem := CMinSel_core_sem).
+  apply CMinSel_forward.
 Defined.
