sepcomp/effect_semantics.v
@@ -1113,11 +1113,16 @@ Proof. intros.
   rewrite PMap.gso. trivial. intros N; subst. elim n; trivial. 
 Qed.
 
-Axiom BuiltinEffect : forall {F V: Type} (ge: Genv.t F V) (sg: signature) 
+Parameter BuiltinEffect : forall {F V: Type} (ge: Genv.t F V) (sg: signature) 
                     (vargs:list val) (m:mem), block -> Z -> bool.
-
+(*
 Axiom BUILTIN: forall (name: ident) (F V: Type) (ge: Genv.t F V) (sg: signature) 
                     (vargs:list val)
                        (m:mem) (t:trace) (v: val) (m': mem),
       extcall_io_sem name sg ge vargs m t v m' ->
       Mem.unchanged_on (fun b z => BuiltinEffect ge sg vargs m b z = false) m m'.
+*)
+Axiom ec_builtinEffectPolymorphic:
+   forall {F V:Type} ef (g : Genv.t F V) vargs m t vres m',
+   external_call ef g vargs m t vres m' ->
+   Mem.unchanged_on (fun b z=> BuiltinEffect g (ef_sig ef) vargs m b z = false) m m'.
